examples/ghc/theories/CoreStats.v
@@ -1,0 +1,9 @@
+Require CoreStats.
+Require Import Proofs.CoreInduct.
+Require Import Omega.
+
+Lemma strictly_greater_than_zero : forall (e: Core.CoreExpr), CoreStats.exprSize e > 0.
+Proof. 
+  intro e.
+  eapply (core_induct e); intros; simpl; omega.
+Qed.  
